Mathematically, if the prior  $p(\theta)$ and the likelihood  $p(x | \theta)$  are such that the posterior  $p(\theta | x)$  is in the same family as  $p(\theta)$ , then  $p(\theta)$  is a conjugate prior for  $p(x | \theta)$.

| Likelihood Function                                                                                                                                                          | Conjugate Prior                                                                                                                                             | Posterior Distribution                                                                                                                                                                                                                                                                  |
| ---------------------------------------------------------------------------------------------------------------------------------------------------------------------------- | ----------------------------------------------------------------------------------------------------------------------------------------------------------- | --------------------------------------------------------------------------------------------------------------------------------------------------------------------------------------------------------------------------------------------------------------------------------------- |
| **Bernoulli/Binomial Distribution**<br> $p(x \mid \theta) = \theta^{x} (1 - \theta)^{n - x}$                                                                                 | **Beta Distribution**<br> $p(\theta) = \dfrac{\theta^{\alpha - 1} (1 - \theta)^{\beta - 1}}{B(\alpha, \beta)}$                                              | **Beta Distribution**<br> $p(\theta \mid x) = \dfrac{\theta^{\alpha' - 1} (1 - \theta)^{\beta' - 1}}{B(\alpha', \beta')}$<br>where $\alpha' = \alpha + x$, $\beta' = \beta + n - x$                                                                                                     |
| **Poisson Distribution**<br> $p(x \mid \lambda) = \dfrac{e^{-\lambda} \lambda^{x}}{x!}$                                                                                      | **Gamma Distribution**<br> $p(\lambda) = \dfrac{\beta^{\alpha}}{\Gamma(\alpha)} \lambda^{\alpha - 1} e^{-\beta \lambda}$                                    | **Gamma Distribution**<br> $p(\lambda \mid x) = \dfrac{(\beta')^{\alpha'}}{\Gamma(\alpha')} \lambda^{\alpha' - 1} e^{-\beta' \lambda}$<br>where $\alpha' = \alpha + \sum x_i$, $\beta' = \beta + n$                                                                                     |
| **Normal Distribution with Known Variance $\sigma^2$**<br> $p(x \mid \mu) = \dfrac{1}{\sqrt{2\pi \sigma^2}} e^{-\dfrac{(x - \mu)^2}{2\sigma^2}}$                             | **Normal Distribution**<br> $p(\mu) = \dfrac{1}{\sqrt{2\pi \tau^2}} e^{-\dfrac{(\mu - \mu_0)^2}{2\tau^2}}$                                                  | **Normal Distribution**<br> $p(\mu \mid x) = \dfrac{1}{\sqrt{2\pi \tau'^2}} e^{-\dfrac{(\mu - \mu')^2}{2\tau'^2}}$<br>where $\tau'^2 = \left( \dfrac{1}{\tau^2} + \dfrac{n}{\sigma^2} \right)^{-1}$, $\mu' = \tau'^2 \left( \dfrac{\mu_0}{\tau^2} + \dfrac{\sum x_i}{\sigma^2} \right)$ |
| **Normal Distribution with Unknown Mean $\mu$ and Known Variance $\sigma^2$**                                                                                                | **Normal-Gamma Distribution**<br>$p(\mu, \lambda) = \text{Normal}(\mu \mid \mu_0, (\lambda \tau^2)^{-1})$ $\times \text{Gamma}(\lambda \mid \alpha, \beta)$ | **Normal-Gamma Distribution**<br> Updated parameters after observing data                                                                                                                                                                                                               |
| **Normal Distribution with Unknown Variance $\sigma^2$ and Known Mean $\mu$**<br> $p(x \mid \sigma^2) = \dfrac{1}{\sqrt{2\pi \sigma^2}} e^{-\dfrac{(x - \mu)^2}{2\sigma^2}}$ | **Inverse-Gamma Distribution**<br> $p(\sigma^2) = \dfrac{\beta^{\alpha}}{\Gamma(\alpha)} (\sigma^2)^{-\alpha - 1} e^{-\dfrac{\beta}{\sigma^2}}$             | **Inverse-Gamma Distribution**<br> $p(\sigma^2 \mid x) = \dfrac{(\beta')^{\alpha'}}{\Gamma(\alpha')} (\sigma^2)^{-\alpha' - 1} e^{-\dfrac{\beta'}{\sigma^2}}$<br>where $\alpha' = \alpha + \dfrac{n}{2}$, $\beta' = \beta + \dfrac{1}{2} \sum (x_i - \mu)^2$                            |
| **Multinomial Distribution**<br> $p(\mathbf{x} \mid \boldsymbol{\theta}) = \dfrac{n!}{\prod_{i} x_i!} \prod_{i} \theta_i^{x_i}$                                              | **Dirichlet Distribution**<br> $p(\boldsymbol{\theta}) = \dfrac{1}{B(\boldsymbol{\alpha})} \prod_{i} \theta_i^{\alpha_i - 1}$                               | **Dirichlet Distribution**<br> $p(\boldsymbol{\theta} \mid \mathbf{x}) = \dfrac{1}{B(\boldsymbol{\alpha}')} \prod_{i} \theta_i^{\alpha_i' - 1}$<br>where $\alpha_i' = \alpha_i + x_i$                                                                                                   |
| **Exponential Distribution**<br> $p(x \mid \lambda) = \lambda e^{-\lambda x}$                                                                                                | **Gamma Distribution**<br> $p(\lambda) = \dfrac{\beta^{\alpha}}{\Gamma(\alpha)} \lambda^{\alpha - 1} e^{-\beta \lambda}$                                    | **Gamma Distribution**<br> $p(\lambda \mid x) = \dfrac{(\beta')^{\alpha'}}{\Gamma(\alpha')} \lambda^{\alpha' - 1} e^{-\beta' \lambda}$<br>where $\alpha' = \alpha + n$, $\beta' = \beta + \sum x_i$                                                                                     |
| **Geometric Distribution**<br> $p(x \mid \theta) = (1 - \theta)^{x} \theta$                                                                                                  | **Beta Distribution**<br> $p(\theta) = \dfrac{\theta^{\alpha - 1} (1 - \theta)^{\beta - 1}}{B(\alpha, \beta)}$                                              | **Beta Distribution**<br> $p(\theta \mid x) = \dfrac{\theta^{\alpha' - 1} (1 - \theta)^{\beta' - 1}}{B(\alpha', \beta')}$<br>where $\alpha' = \alpha + n$, $\beta' = \beta + \sum x_i$                                                                                                  |
| **Negative Binomial Distribution**<br> $p(x \mid r, p) = \dfrac{\Gamma(x + r)}{x! \, \Gamma(r)} p^{r} (1 - p)^{x}$                                                           | **Beta Distribution for $p$**<br> $p(p) = \dfrac{p^{\alpha - 1} (1 - p)^{\beta - 1}}{B(\alpha, \beta)}$                                                     | **Beta Distribution**<br> $p(p \mid x) = \dfrac{p^{\alpha' - 1} (1 - p)^{\beta' - 1}}{B(\alpha', \beta')}$<br>where $\alpha' = \alpha + r n$, $\beta' = \beta + \sum x_i$                                                                                                               |
