### **Reciprocal Identities**
$$
\sin \theta = \frac{1}{\csc \theta}, \quad \csc \theta = \frac{1}{\sin \theta}
$$
$$
\cos \theta = \frac{1}{\sec \theta}, \quad \sec \theta = \frac{1}{\cos \theta}
$$
$$
\tan \theta = \frac{1}{\cot \theta}, \quad \cot \theta = \frac{1}{\tan \theta}
$$

### **Pythagorean Identities**
$$
\sin^2 \theta + \cos^2 \theta = 1
$$
$$
1 + \tan^2 \theta = \sec^2 \theta
$$
$$
1 + \cot^2 \theta = \csc^2 \theta
$$

### **Quotient Identities**
$$
\tan \theta = \frac{\sin \theta}{\cos \theta}
$$
$$
\cot \theta = \frac{\cos \theta}{\sin \theta}
$$

### **Co-Function Identities**
$$
\sin \left(\frac{\pi}{2} - \theta\right) = \cos \theta, \quad \cos \left(\frac{\pi}{2} - \theta\right) = \sin \theta
$$
$$
\tan \left(\frac{\pi}{2} - \theta\right) = \cot \theta, \quad \cot \left(\frac{\pi}{2} - \theta\right) = \tan \theta
$$
$$
\sec \left(\frac{\pi}{2} - \theta\right) = \csc \theta, \quad \csc \left(\frac{\pi}{2} - \theta\right) = \sec \theta
$$

### **Even-Odd Identities**
$$
\sin(-\theta) = -\sin \theta
$$
$$
\cos(-\theta) = \cos \theta
$$
$$
\tan(-\theta) = -\tan \theta
$$
$$
\csc(-\theta) = -\csc \theta
$$
$$
\sec(-\theta) = \sec \theta
$$
$$
\cot(-\theta) = -\cot \theta
$$

### **Sum and Difference Identities**
$$
\sin(\alpha \pm \beta) = \sin \alpha \cos \beta \pm \cos \alpha \sin \beta
$$
$$
\cos(\alpha \pm \beta) = \cos \alpha \cos \beta \mp \sin \alpha \sin \beta
$$
$$
\tan(\alpha \pm \beta) = \frac{\tan \alpha \pm \tan \beta}{1 \mp \tan \alpha \tan \beta}
$$

### **Double Angle Identities**
$$
\sin(2\theta) = 2 \sin \theta \cos \theta
$$
$$
\cos(2\theta) = \cos^2 \theta - \sin^2 \theta = 2\cos^2 \theta - 1 = 1 - 2\sin^2 \theta
$$
$$
\tan(2\theta) = \frac{2\tan \theta}{1 - \tan^2 \theta}
$$

### **Half Angle Identities**
$$
\sin\left(\frac{\theta}{2}\right) = \pm \sqrt{\frac{1 - \cos \theta}{2}}
$$
$$
\cos\left(\frac{\theta}{2}\right) = \pm \sqrt{\frac{1 + \cos \theta}{2}}
$$
$$
\tan\left(\frac{\theta}{2}\right) = \pm \sqrt{\frac{1 - \cos \theta}{1 + \cos \theta}} = \frac{\sin \theta}{1 + \cos \theta} = \frac{1 - \cos \theta}{\sin \theta}
$$

### **Product-to-Sum Identities**
$$
\sin \alpha \sin \beta = \frac{1}{2} [\cos(\alpha - \beta) - \cos(\alpha + \beta)]
$$
$$
\cos \alpha \cos \beta = \frac{1}{2} [\cos(\alpha + \beta) + \cos(\alpha - \beta)]
$$
$$
\sin \alpha \cos \beta = \frac{1}{2} [\sin(\alpha + \beta) + \sin(\alpha - \beta)]
$$

### **Sum-to-Product Identities**
$$
\sin \alpha + \sin \beta = 2 \sin\left(\frac{\alpha + \beta}{2}\right) \cos\left(\frac{\alpha - \beta}{2}\right)
$$
$$
\sin \alpha - \sin \beta = 2 \cos\left(\frac{\alpha + \beta}{2}\right) \sin\left(\frac{\alpha - \beta}{2}\right)
$$
$$
\cos \alpha + \cos \beta = 2 \cos\left(\frac{\alpha + \beta}{2}\right) \cos\left(\frac{\alpha - \beta}{2}\right)
$$
$$
\cos \alpha - \cos \beta = -2 \sin\left(\frac{\alpha + \beta}{2}\right) \sin\left(\frac{\alpha - \beta}{2}\right)
$$
### Reciprocal trigonometric functions
